src/InlineFacts_2.v
@@ -414,172 +414,6 @@ Proof.
       admit. (* induction case: after UnitSteps semantics are changed *)
 Qed.
 
-Lemma inlineDmToMod_correct_UnitSteps:
-  forall m (Hm: BasicMod m) (Hequiv: ModEquiv typeUT type m)
-         or nr l dm,
-    NoDup (namesOf (getDmsBodies m)) ->
-    UnitSteps m or nr l ->
-    M.find dm (dms l) = M.find dm (cms l) ->
-    snd (inlineDmToMod m dm) = true ->
-    UnitSteps (fst (inlineDmToMod m dm)) or nr (hideMeth l dm).
-Proof.
-  induction 4; intros; [constructor; apply inlineDmToMod_correct_UnitStep_1; auto|].
-
-  destruct l1 as [rm1 dm1 cm1], l2 as [rm2 dm2 cm2]; simpl in *.
-  remember (M.find dm (M.union dm1 dm2)) as odmv.
-  destruct odmv.
-
-  - unfold inlineDmToMod, hideMeth in *; simpl in *.
-    rewrite <-Heqodmv, <-H0; simpl.
-    destruct (signIsEq t t); [clear e|elim n; auto].
-
-    remember (wfModules m) as owf; destruct owf; [|discriminate].
-    remember (getAttribute dm (getDmsBodies m)) as odm; destruct odm; [|discriminate].
-    remember (noCallDm a a) as oc; destruct oc; [|discriminate].
-
-    pose proof (getAttribute_Some_name _ _ Heqodm); subst.
-    destruct m as [regs rules dms|]; [|exfalso; inv Hm].
-
-    unfold CanCombine in c; dest; simpl in *.
-    rewrite M.find_union in Heqodmv; rewrite M.find_union in H0.
-    remember (M.find a dm1) as odmv1; destruct odmv1.
-    
-    + inv Heqodmv.
-      remember (M.find a cm1) as ocmv1; destruct ocmv1.
-      * (* left-side inlined *)
-        inv H0; specialize (IHX1 eq_refl).
-        destruct (signIsEq t t); [clear e|elim n; auto].
-
-        do 2 rewrite M.remove_union.
-        match goal with
-          | [ |- UnitSteps _ _ _ ?l ] =>
-            replace l with
-            (mergeLabel {| ruleMeth:= rm1;
-                           dms:= M.remove a dm1;
-                           cms:= M.remove a cm1 |}
-                        {| ruleMeth:= rm2;
-                           dms:= M.remove a dm2;
-                           cms:= M.remove a cm2 |})
-              by reflexivity
-        end.
-        apply UnitStepsUnion; auto.
-        { assert (M.find a dm2 = None)
-            by (destruct (M.Disj_find_None a H4); auto;
-                rewrite H0 in Heqodmv1; inv Heqodmv1).
-          assert (M.find a cm2 = None)
-            by (destruct (M.Disj_find_None a H5); auto;
-                rewrite H6 in Heqocmv1; inv Heqocmv1).
-          do 2 rewrite M.remove_find_None by assumption.
-          eapply inlineDmToRules_UnitSteps_intact; eauto.
-          eapply inlineDmToDms_UnitSteps_intact; eauto.
-          apply wfModules_WfModules; auto.
-        }
-        { repeat split; simpl; auto.
-          { apply M.Disj_remove_1, M.Disj_remove_2; assumption. }
-          { apply M.Disj_remove_1, M.Disj_remove_2; assumption. }
-        }
-
-      * pose proof (getAttribute_Some_body _ _ Heqodm).
-        eapply inlineDmToMod_correct_UnitSteps_sub; eauto.
-        apply wfModules_WfModules; auto.
-        
-    + remember (M.find a cm1) as ocmv1; destruct ocmv1.
-      * clear IHX1 IHX2; inv H0.
-        replace (M.union u1 u2) with (M.union u2 u1)
-          by (apply M.union_comm; apply M.Disj_comm; auto).
-        replace (match rm1 with | Some r => Some r | None => rm2 end) with
-        (match rm2 with | Some r => Some r | None => rm1 end)
-          by (destruct rm1, rm2; intuition idtac; destruct H3; discriminate).
-        replace (M.union dm1 dm2) with (M.union dm2 dm1)
-          by (apply M.union_comm; apply M.Disj_comm; auto).
-        replace (M.union cm1 cm2) with (M.union cm2 cm1)
-          by (apply M.union_comm; apply M.Disj_comm; auto).
-        pose proof (getAttribute_Some_body _ _ Heqodm).
-        eapply inlineDmToMod_correct_UnitSteps_sub; eauto; try (apply M.Disj_comm; auto).
-        { apply wfModules_WfModules; auto. }
-        { destruct H3; unfold NotBothRule; intuition auto. }
-      * (* right-side inlined *)
-        rewrite <-Heqodmv, <-H0 in IHX2.
-        specialize (IHX2 eq_refl).
-        destruct (signIsEq t t); [clear e|elim n; auto].
-
-        do 2 rewrite M.remove_union.
-        match goal with
-          | [ |- UnitSteps _ _ _ ?l ] =>
-            replace l with
-            (mergeLabel {| ruleMeth:= rm1;
-                           dms:= M.remove a dm1;
-                           cms:= M.remove a cm1 |}
-                        {| ruleMeth:= rm2;
-                           dms:= M.remove a dm2;
-                           cms:= M.remove a cm2 |})
-              by reflexivity
-        end.
-        apply UnitStepsUnion; auto.
-        { do 2 rewrite M.remove_find_None by auto.
-          eapply inlineDmToRules_UnitSteps_intact; eauto.
-          eapply inlineDmToDms_UnitSteps_intact; eauto.
-          apply wfModules_WfModules; auto.
-        }
-        { repeat split; simpl; auto.
-          { apply M.Disj_remove_1, M.Disj_remove_2; assumption. }
-          { apply M.Disj_remove_1, M.Disj_remove_2; assumption. }
-        }
-
-  - unfold inlineDmToMod, hideMeth in *; simpl in *; rewrite <-Heqodmv.
-    rewrite M.find_union in Heqodmv.
-    destruct (M.find dm dm1); [discriminate|].
-    destruct (M.find dm dm2); [discriminate|].
-    rewrite M.find_union in H0.
-    destruct (M.find dm cm1); [discriminate|].
-    destruct (M.find dm cm2); [discriminate|].
-    specialize (IHX1 eq_refl); specialize (IHX2 eq_refl).
-
-    destruct (wfModules m); [|discriminate].
-    destruct (getAttribute dm (getDmsBodies m)); [|discriminate].
-    destruct (noCallDm a a); [|discriminate].
-    destruct m; [|discriminate].
-    simpl in *.
-    specialize (IHX1 eq_refl); specialize (IHX2 eq_refl).
-    apply (UnitStepsUnion IHX1 IHX2 c).
-Qed.
-
-Lemma inlineDmToMod_getDmsMod:
-  forall m a,
-    getDmsMod m = getDmsMod (fst (inlineDmToMod m a)).
-Proof.
-  intros; unfold inlineDmToMod.
-  destruct (wfModules _); [|auto].
-  destruct (getAttribute _ _); [|auto].
-  destruct (noCallDm _ _); [|auto].
-  destruct m; [|auto].
-  simpl.
-
-  clear; induction dms; [auto|].
-  simpl; f_equal; auto.
-Qed.
-
-Lemma inlineDmToMod_wellHidden:
-  forall {A} (l: LabelTP A) m a,
-    wellHidden l m ->
-    wellHidden l (fst (inlineDmToMod m a)).
-Proof.
-  unfold wellHidden; intros.
-  rewrite <-inlineDmToMod_getDmsMod.
-  admit.
-Qed.
-
-Lemma wellHidden_find:
-  forall {A} m a (l: LabelTP A),
-    In a (namesOf (getDmsBodies m)) ->
-    wellHidden (hide l) m ->
-    M.find a (dms l) = M.find a (cms l).
-Proof.
-  unfold wellHidden, hide; intros.
-  destruct l as [rm dm cm]; simpl in *.
-  admit. (* a bit complicated map stuff *)
-Qed.
-
 Lemma inlineDmToMod_basicMod:
   forall m a,
     BasicMod m ->
@@ -590,23 +424,107 @@ Proof.
   auto.
 Qed.
 
-Lemma inlineDmToMod_dms_names:
-  forall m a,
-    namesOf (getDmsBodies (fst (inlineDmToMod m a))) =
-    namesOf (getDmsBodies m).
+Definition InlinableDm (m: Modules) (dm: string) :=
+  match getAttribute dm (getDefsBodies m) with
+    | Some dmb =>
+      if noCallDm dmb dmb then True else False
+    | _ => False
+  end.
+
+ *)
+
+Lemma hideMeths_hide:
+  forall dmsAll (l: LabelT),
+    M.KeysSubset (defs l) dmsAll ->
+    hideMeths l dmsAll = hide l.
 Proof.
-  destruct m; intros; simpl in *.
-  - unfold inlineDmToMod.
-    destruct (wfModules _); try destruct (getAttribute _ _); try destruct (noCallDm _ _);
-    try (reflexivity; fail).
-    simpl; clear.
+  induction dmsAll; intros.
 
-    induction dms; auto.
-    simpl; f_equal; auto.
+  - destruct l as [rm dm cm]; simpl in *.
+    rewrite (M.KeysSubset_nil H).
+    unfold hide; simpl.
+    f_equal; auto.
+    rewrite M.subtractKV_empty_1; reflexivity.
 
-  - unfold inlineDmToMod.
-    destruct (wfModules _); try destruct (getAttribute _ _); try destruct (noCallDm _ _);
-    reflexivity.
+  - destruct l as [rm dm cm]; simpl in *.
+    remember (M.find a dm) as oda; remember (M.find a cm) as oca.
+    destruct oda.
+    + destruct oca.
+      * unfold hideMeth; simpl.
+        rewrite <-Heqoda, <-Heqoca.
+        destruct (signIsEq s s0).
+        { subst; rewrite IHdmsAll.
+          { unfold hide; f_equal; auto; apply M.subtractKV_remove; simpl;
+            rewrite <-Heqoda, <-Heqoca; auto.
+          }
+          { simpl; apply M.KeysSubset_remove; auto. }
+        }
+        { admit. (* a bit complicated map stuff *) }
+
+      * unfold hideMeth; simpl.
+        rewrite <-Heqoda, <-Heqoca.
+        admit. (* same as above *)
+
+    + unfold hideMeth; simpl.
+      rewrite <-Heqoda.
+      rewrite IHdmsAll; simpl; [reflexivity|].
+      eapply M.KeysSubset_find_None; eauto.
+Qed.
+
+Lemma inlineDmToMod_getDmsMod:
+  forall m a,
+    getDefs m = getDefs (fst (inlineDmToMod m a)).
+Proof.
+  intros; unfold inlineDmToMod.
+  destruct (wfModules _); [|auto].
+  destruct (getAttribute _ _); [|auto].
+  destruct (noCallDm _ _); [|auto].
+  destruct m; [|auto].
+  simpl.
+
+  clear; induction dms; [auto|].
+  unfold getDefs; simpl.
+  simpl; f_equal; auto.
+Qed.
+
+Lemma inlineDmToMod_wellHidden:
+  forall m (l: LabelT) a,
+    wellHidden m l ->
+    wellHidden (fst (inlineDmToMod m a)) l.
+Proof.
+  unfold wellHidden; intros.
+  rewrite <-inlineDmToMod_getDmsMod.
+  admit. (* a nontrivial proof about getCalls *)
+Qed.
+
+Lemma inlineDms_wellHidden:
+  forall m (l: LabelT),
+    wellHidden m l ->
+    wellHidden (fst (inlineDms m)) l.
+Proof.
+  intros; unfold inlineDms.
+  remember (namesOf (getDefsBodies m)) as dms; clear Heqdms.
+  generalize dependent m; induction dms; intros; [assumption|].
+  simpl; remember (inlineDmToMod m a) as imb; destruct imb; simpl.
+  destruct b.
+  - apply IHdms; auto.
+    replace m0 with (fst (inlineDmToMod m a)) by (rewrite <-Heqimb; reflexivity).
+    apply inlineDmToMod_wellHidden; auto.
+  - unfold inlineDmToMod in Heqimb.
+    destruct (wfModules _); [|inv Heqimb; assumption].
+    destruct (getAttribute _ _); [|inv Heqimb; assumption].
+    destruct (noCallDm _ _); [|inv Heqimb; assumption].
+    destruct m; [|inv Heqimb; assumption].
+    inv Heqimb.
+Qed.
+
+Lemma hideMeths_UnitSteps_hide:
+  forall m or nr l,
+    SubstepsInd m or nr l ->
+    hideMeths l (namesOf (getDefsBodies m)) = hide l.
+Proof.
+  intros; apply hideMeths_hide.
+  admit. (* Semantics proof: dyn dms <= static dms *)
 Qed.
 
 Lemma inlineDm_ActionEquiv:
@@ -615,7 +533,7 @@ Lemma inlineDm_ActionEquiv:
     (forall (argV1: ft1 type1 (SyntaxKind _))
             (argV2: ft2 type2 (SyntaxKind _)),
        ActionEquiv (vars (argV1, argV2) :: nil)
-                   (objVal (attrType dm) type1 argV1) (objVal (attrType dm) type2 argV2)) ->
+                   (projT2 (attrType dm) type1 argV1) (projT2 (attrType dm) type2 argV2)) ->
     ActionEquiv G aU aT ->
     ActionEquiv G (inlineDm aU dm) (inlineDm aT dm).
 Proof.
@@ -642,7 +560,7 @@ Lemma inlineDmToRules_RulesEquiv:
     (forall (argV1: ft1 type1 (SyntaxKind _))
             (argV2: ft2 type2 (SyntaxKind _)),
        ActionEquiv (vars (argV1, argV2) :: nil)
-                   (objVal (attrType dm) type1 argV1) (objVal (attrType dm) type2 argV2)) ->
+                   (projT2 (attrType dm) type1 argV1) (projT2 (attrType dm) type2 argV2)) ->
     RulesEquiv type1 type2 rules ->
     RulesEquiv type1 type2 (inlineDmToRules rules dm).
 Proof.
@@ -655,7 +573,7 @@ Lemma inlineDmToDms_MethsEquiv:
     (forall (argV1: ft1 type1 (SyntaxKind _))
             (argV2: ft2 type2 (SyntaxKind _)),
        ActionEquiv (vars (argV1, argV2) :: nil)
-                   (objVal (attrType dm) type1 argV1) (objVal (attrType dm) type2 argV2)) ->
+                   (projT2 (attrType dm) type1 argV1) (projT2 (attrType dm) type2 argV2)) ->
     MethsEquiv type1 type2 dms ->
     MethsEquiv type1 type2 (inlineDmToDms dms dm).
 Proof.
@@ -687,16 +605,58 @@ Proof.
     auto.
 Qed.
 
+Lemma inlineDmToMod_dms_names:
+  forall m a,
+    namesOf (getDefsBodies (fst (inlineDmToMod m a))) =
+    namesOf (getDefsBodies m).
+Proof.
+  destruct m; intros; simpl in *.
+  - unfold inlineDmToMod.
+    destruct (wfModules _); try destruct (getAttribute _ _); try destruct (noCallDm _ _);
+    try (reflexivity; fail).
+    simpl; clear.
+
+    induction dms; auto.
+    simpl; f_equal; auto.
+
+  - unfold inlineDmToMod.
+    destruct (wfModules _); try destruct (getAttribute _ _); try destruct (noCallDm _ _);
+    reflexivity.
+Qed.
+
+Lemma inlineDmToMod_correct_UnitSteps:
+  forall m (Hequiv: ModEquiv typeUT type m)
+         or nr l dm,
+    NoDup (namesOf (getDefsBodies m)) ->
+    SubstepsInd m or nr l ->
+    M.find dm (defs l) = M.find dm (calls l) ->
+    snd (inlineDmToMod m dm) = true ->
+    SubstepsInd (fst (inlineDmToMod m dm)) or nr (hideMeth l dm).
+Proof.
+  induction 3; intros; [constructor|].
+  admit.
+Qed.
+
+Lemma wellHidden_find:
+  forall m a (l: LabelT),
+    In a (namesOf (getDefsBodies m)) ->
+    wellHidden m (hide l) ->
+    M.find a (defs l) = M.find a (calls l).
+Proof.
+  unfold wellHidden, hide; intros.
+  destruct l as [rm dm cm]; simpl in *.
+  admit. (* a bit complicated map stuff *)
+Qed.
+
 Lemma inlineDms'_correct_UnitSteps:
-  forall cdms m (Hm: BasicMod m)
-         (Hequiv: ModEquiv typeUT type m)
-         (Hdms: NoDup (namesOf (getDmsBodies m)))
-         (Hcdms: SubList cdms (namesOf (getDmsBodies m)))
+  forall cdms m (Hequiv: ModEquiv typeUT type m)
+         (Hdms: NoDup (namesOf (getDefsBodies m)))
+         (Hcdms: SubList cdms (namesOf (getDefsBodies m)))
          or nr l,
-    UnitSteps m or nr l ->
-    wellHidden (hide l) m ->
+    SubstepsInd m or nr l ->
+    wellHidden m (hide l) ->
     snd (inlineDms' m cdms) = true ->
-    UnitSteps (fst (inlineDms' m cdms)) or nr (hideMeths l cdms).
+    SubstepsInd (fst (inlineDms' m cdms)) or nr (hideMeths l cdms).
 Proof.
   induction cdms; [auto|].
   intros; simpl.
@@ -706,7 +666,6 @@ Proof.
 
   - assert (im = fst (inlineDmToMod m a)) by (rewrite <-Heqimb; reflexivity); subst.
     apply IHcdms; auto.
-    + eapply inlineDmToMod_basicMod; eauto.
     + apply inlineDmToMod_ModEquiv; auto.
     + rewrite inlineDmToMod_dms_names; auto.
     + rewrite inlineDmToMod_dms_names; auto.
@@ -716,7 +675,7 @@ Proof.
         destruct b; [auto|inv Heqimb].
     + apply inlineDmToMod_wellHidden.
       rewrite hideMeth_preserves_hide; auto.
-    + simpl in H0; destruct (inlineDmToMod m a); simpl in *.
+    + simpl in H1; destruct (inlineDmToMod m a); simpl in *.
       destruct b; [auto|inv Heqimb].
 
   - simpl in *; unfold inlineDmToMod in *.
@@ -727,67 +686,13 @@ Proof.
     inv Heqimb.
 Qed.
 
-Lemma hideMeths_hide:
-  forall dmsAll {A} (l: LabelTP A),
-    M.KeysSubset (dms l) dmsAll ->
-    hideMeths l dmsAll = hide l.
-Proof.
-  induction dmsAll; intros.
-
-  - destruct l as [rm dm cm]; simpl in *.
-    rewrite (M.KeysSubset_nil _ H).
-    f_equal; auto.
-    rewrite M.subtractKV_empty_1; reflexivity.
-
-  - destruct l as [rm dm cm]; simpl in *.
-    remember (M.find a dm) as oda; remember (M.find a cm) as oca.
-    destruct oda.
-    + destruct oca.
-      * unfold hideMeth; simpl.
-        rewrite <-Heqoda, <-Heqoca.
-        destruct (signIsEq t t0).
-        { subst; rewrite IHdmsAll.
-          { unfold hide; f_equal; auto; apply M.subtractKV_remove;
-            rewrite <-Heqoda, <-Heqoca; auto.
-          }
-          { simpl; apply M.KeysSubset_remove; auto. }
-        }
-        { admit. (* a bit complicated map stuff *) }
-
-      * unfold hideMeth; simpl.
-        rewrite <-Heqoda, <-Heqoca.
-        admit. (* same as above *)
-
-    + unfold hideMeth; simpl.
-      rewrite <-Heqoda.
-      rewrite IHdmsAll; simpl; [reflexivity|].
-      eapply M.KeysSubset_find_None; eauto.
-Qed.
-
-Lemma hideMeths_UnitSteps_hide:
-  forall m or nr l,
-    UnitSteps m or nr l ->
-    hideMeths l (namesOf (getDmsBodies m)) = hide l.
-Proof.
-  intros; apply hideMeths_hide.
-  admit. (* Semantics proof: dyn dms <= static dms *)
-Qed.
-
-Definition InlinableDm (m: Modules) (dm: string) :=
-  match getAttribute dm (getDmsBodies m) with
-    | Some dmb =>
-      if noCallDm dmb dmb then True else False
-    | _ => False
-  end.
-
-Lemma inlineDms_correct_UnitSteps:
-  forall m (Hm: BasicMod m)
-         (Hequiv: ModEquiv typeUT type m)
-         (Hdms: NoDup (namesOf (getDmsBodies m))) or nr l,
-    UnitSteps m or nr l ->
+Lemma inlineDms_correct_SubstepsInd:
+  forall m (Hequiv: ModEquiv typeUT type m)
+         (Hdms: NoDup (namesOf (getDefsBodies m))) or u l,
+    SubstepsInd m or u l ->
     snd (inlineDms m) = true ->
-    wellHidden (hide l) m ->
-    UnitSteps (fst (inlineDms m)) or nr (hide l).
+    wellHidden m (hide l) ->
+    SubstepsInd (fst (inlineDms m)) or u (hide l).
 Proof.
   intros.
   erewrite <-hideMeths_UnitSteps_hide; eauto.
@@ -795,80 +700,41 @@ Proof.
   apply SubList_refl.
 Qed.
 
-Lemma inlineDms_wellHidden:
-  forall {A} (l: LabelTP A) m,
-    wellHidden l m ->
-    wellHidden l (fst (inlineDms m)).
-Proof.
-  intros; unfold inlineDms.
-  remember (namesOf (getDmsBodies m)) as dms; clear Heqdms.
-  generalize dependent m; induction dms; intros; [assumption|].
-  simpl; remember (inlineDmToMod m a) as imb; destruct imb; simpl.
-  destruct b.
-  - apply IHdms; auto.
-    replace m0 with (fst (inlineDmToMod m a)) by (rewrite <-Heqimb; reflexivity).
-    apply inlineDmToMod_wellHidden; auto.
-  - unfold inlineDmToMod in Heqimb.
-    destruct (wfModules _); [|inv Heqimb; assumption].
-    destruct (getAttribute _ _); [|inv Heqimb; assumption].
-    destruct (noCallDm _ _); [|inv Heqimb; assumption].
-    destruct m; [|inv Heqimb; assumption].
-    inv Heqimb.
-Qed.
-
 Lemma hide_idempotent:
-  forall {A} (l: LabelTP A), hide l = hide (hide l).
+  forall (l: LabelT), hide l = hide (hide l).
 Proof.
   admit. (* Semantics proof *)
 Qed.
 
-Lemma merge_preserves_step:
-  forall m or nr l,
-    Step m or nr l ->
-    Step (merge m) or nr l.
+Lemma inlineDms_correct:
+  forall m (Hequiv: ModEquiv typeUT type m)
+         (Hdms: NoDup (namesOf (getDefsBodies m)))
+         (Hin: snd (inlineDms m) = true)
+         or nr l,
+    StepInd m or nr l ->
+    StepInd (fst (inlineDms m)) or nr l.
 Proof.
-  admit. (* Semantics proof *)
+  intros; inv H.
+  rewrite hide_idempotent.
+  constructor.
+  - apply inlineDms_correct_SubstepsInd; auto.
+  - rewrite <-hide_idempotent.
+    apply inlineDms_wellHidden; auto.
 Qed.
-
-(* Lemma filter_preserves_step: *)
-(*   forall regs rules dmsAll or nr l filt, *)
-(*     Step (Mod regs rules dmsAll) or nr l -> *)
-(*     M.KeysDisj (dms l) filt -> *)
-(*     Step (Mod regs rules (filterDms dmsAll filt)) or nr l. *)
-(* Proof. *)
-(* Qed. *)
 
 (* Instead of filter, use below *)
 Lemma step_dms_hidden:
   forall m or nr l,
     Step m or nr l ->
-    M.KeysDisj (dms l) (getCmsMod m).
+    M.KeysDisj (defs l) (Syntax.getCalls m).
 Proof.
-  intros; inv X.
-  unfold wellHidden in H0.
-  destruct (hide l0); simpl in *; intuition.
+  intros; inv H.
+  unfold wellHidden in HWellHidden.
+  destruct (hide _); simpl in *; intuition.
 Qed.
- *)
-
-Lemma inlineDms_correct:
-  forall m (Hm: BasicMod m)
-         (Hequiv: ModEquiv typeUT type m)
-         (Hdms: NoDup (namesOf (getDefsBodies m)))
-         (Hin: snd (inlineDms m) = true)
-         or nr l,
-    Step m or nr l ->
-    Step (fst (inlineDms m)) or nr l.
-Proof.
-  induction 5; intros; subst.
-  apply StepIntro with (m := fst (inlineDms m)); auto.
-  - apply inlineDms_correct_UnitSteps; auto.
-  - apply hide_idempotent.
-  - apply inlineDms_wellHidden; auto.
-Qed.
-
 
 Theorem inline_correct:
-  forall m (Hequiv: ModEquiv typeUT type (merge m))
+  forall m (Hequiv: ModEquiv typeUT type m)
          (Hdms: NoDup (namesOf (getDefsBodies m)))
          (Hin: snd (inline m) = true)
          or nr l,
@@ -876,8 +742,7 @@ Theorem inline_correct:
     Step (fst (inline m)) or nr l.
 Proof.
   intros; unfold inline.
+  apply step_consistent; apply step_consistent in H.
   apply inlineDms_correct; auto.
-  - unfold BasicMod, merge; auto.
-  - apply merge_preserves_step; auto.
 Qed.
 
